@prefix :      <http://purl.org/roh/university-hr/es#> .
@prefix geo: <http://purl.org/hercules/asio/modules#> .
@prefix ns:    <http://www.w3.org/2003/06/sw-vocab-status/ns#> .
@prefix owl:   <http://www.w3.org/2002/07/owl#> .
@prefix xsd:   <http://www.w3.org/2001/XMLSchema#> .
@prefix unescothes: <http://skos.um.es/unescothes/> .
@prefix skos:  <http://www.w3.org/2004/02/skos/core#> .
@prefix rdfs:  <http://www.w3.org/2000/01/rdf-schema#> .
@prefix terms: <http://purl.org/dc/terms/> .
@prefix rdf:   <http://www.w3.org/1999/02/22-rdf-syntax-ns#> .
@prefix euCountry: <http://publications.europa.eu/resource/authority/country/> .
@prefix vivo:  <http://purl.org/roh/mirror/vivo#> .
@prefix roh:   <http://purl.org/roh#> .
@prefix rohuk: <http://purl.org/roh/university-hr/uk#> .
@prefix rohpt: <http://purl.org/roh/university-hr/pt#> .

<http://purl.org/roh/university-hr/es>
        a               owl:Ontology ;
	rdfs:label      "ROH Spanish University HR Module"@en ;
        rdfs:comment    "The University of Murcia signed on November 29, 2017, a Covenant with the Ministry of Economy, Industry and Competitiveness backing the “HÉRCULES: Semantic University Research Data” Project with a budget of FIVE MILLION FOUR HUNDRED AND SIXTY-TWO THOUSAND SIX HUNDRED euros with an 80% of co-financiering from the European Regional Development Fund program (ERDF) within the 2014-2020 period. \n\nThe project arose as a CRUE initiative, to create the basis for a new collaboration model between universities, to develop the information management systems and with the main objective of encouraging this type of collaboration.\n\nTherefore, the purpose of this agreement was to contribute to the improvement of public services and business innovation and research through the improvement of:\n\n    efficiency in public investment by decreasing the duplication of investment in R&D.\n    efficiency of research in universities.\n    scientific dissemination of research results.\n    detection of synergies in R&D between universities.\n    transfer of R&D results to companies.\n    efficiency in the management of research. \n\nby creating a research management system with semantic capacities based on semantic open data and that will provide a global view of the research data contained in the Spanish University System."@en ;
        terms:license   <https://creativecommons.org/licenses/by-sa/4.0/> ;
        owl:versionIRI  <http://purl.org/roh/university-hr/1.0> .

roh:geoDivision a owl:AnnotationProperty .

vivo:Position  a         owl:Class ;
	rdfs:label       "Position"@en , "Posición"@es .

vivo:FacultyPosition  a  owl:Class ;
        rdfs:label       "Faculty Position"@en , "Posición en Facultad"@es ;
	rdfs:subClassOf  vivo:Position .

vivo:NonAcademicPosition
        a       owl:Class ;
	rdfs:label "Non-Academic Position"@en , "Posición no Académica"@es ;
	rdfs:subClassOf  vivo:Position .

vivo:NonFacultyAcademicPosition
        a                owl:Class ;
        rdfs:label       "Non-Faculty Academic Position"@en , "Posición Académica no de Facultad"@es ;
        rdfs:subClassOf  vivo:Position .

vivo:FacultyAdministrativePosition
        a                owl:Class ;
        rdfs:label       "Faculty Administrative Position"@en , "Posición Administrativa en Facultad"@es ;
        rdfs:subClassOf  vivo:Position .

skos:Concept
        a       owl:Class ;
	rdfs:label "Concept"@en .

skos:ConceptScheme
        a       owl:Class ;
	rdfs:label "Concept Scheme"@en .

:ES_UNIVERSITY_HR_ESLPI
        a                owl:Class ;
        rdfs:label       "Profesor laboral interino"@es ;
        rdfs:subClassOf  :PDIContratado ;
        roh:country     euCountry:ESP ;
        roh:hasCode     :ES_UNIVERSITY_HR_CODE_ESLPI ;
        skos:closeMatch  unescothes:C00015 , unescothes:C03965 ;
        skos:inScheme    :ESUniversityHumanResourcesList ;
        skos:notation    "ESLPI" ;
        skos:prefLabel   "Profesor llaboral interín"@ast , "Professor laboral interí"@ca , "Lan kontratudun bitarteko irakaslea"@eu , "Profesor laboral interino"@gl , "Profesor laboral interino"@es .

:ES_UNIVERSITY_HR_ESFIVEFP
        a                 owl:Class ;
        rdfs:label        "Profesor Ivef permanente"@es ;
        rdfs:subClassOf   :CuerpoDocente ;
        roh:country      euCountry:ESP ;
        roh:geoDivision  geo:ES_DIVISION_LEVEL_1_ES_PV ;
        roh:hasCode      :ES_UNIVERSITY_HR_CODE_ESFIVEFP ;
        skos:closeMatch   unescothes:C03965 , unescothes:C00015 ;
        skos:inScheme     :ESUniversityHumanResourcesList ;
        skos:notation     "ESFIVEFP" ;
        skos:prefLabel    "Professor Ivef permanent"@ca , "SHEE Irakaslea (Iraunkorra)"@eu , "Profesor Ivef permanente"@gl , "Profesor Ivef permanente"@ast , "Profesor Ivef permanente"@es .

:ES_UNIVERSITY_HR_ESJEFDEP
        a                owl:Class ;
        rdfs:label       "Director de departamento"@es ;
        rdfs:subClassOf  vivo:FacultyAdministrativePosition ;
        roh:country     euCountry:ESP ;
        roh:hasCode     :ES_UNIVERSITY_HR_CODE_ESJEFDEP ;
        skos:closeMatch  rohuk:GB_UNIVERSITY_GBHEADDEP ;
        skos:inScheme    :ESUniversityHumanResourcesList ;
        skos:notation    "ESJEFDEP" ;
        skos:prefLabel   "Director de departamentu"@ast , "Director de departament"@ca , "Director de departamento"@gl , "Director de departamento"@es , "Saileko Zuzendaria"@eu .

:ES_UNIVERSITY_HR_CODE_ESPASF
        a               skos:Concept ;
        rdfs:label      "ESPASF" ;
        roh:codeOf     :ES_UNIVERSITY_HR_ESPASF ;
        skos:inScheme   :ESUniversityHumanResourcesCodesList ;
        skos:prefLabel  "ESPASF" .

:ES_UNIVERSITY_HR_CODE_ESLPAD
        a               skos:Concept ;
        rdfs:label      "ESLPAD" ;
        roh:codeOf     :ProfesorAyudanteDoctor ;
        skos:inScheme   :ESUniversityHumanResourcesCodesList ;
        skos:prefLabel  "ESLPAD" .

:ES_UNIVERSITY_HR_ESVIDEC
        a                owl:Class ;
        rdfs:label       "Vicedecano"@es ;
        rdfs:subClassOf  vivo:FacultyAdministrativePosition ;
        roh:country     euCountry:ESP ;
        roh:hasCode     :ES_UNIVERSITY_HR_CODE_ESVIDEC ;
        skos:inScheme    :ESUniversityHumanResourcesList ;
        skos:notation    "ESVIDEC" ;
        skos:prefLabel   "Dekanordea"@eu , "Vicedecanu"@ast , "Vicedegà"@ca , "Vicedecano"@es , "Vicedecano"@gl .

:ProfesorAyudanteDoctor
        a                owl:Class ;
        rdfs:comment     "La contratación de Profesoras y Profesores Ayudantes Doctores se ajustará a las siguientes reglas:\na) El contrato se celebrará con doctores. La contratación exigirá la previa evaluación positiva de su actividad por parte de la Agencia Nacional de Evaluación de la Calidad y Acreditación o del órgano de evaluación externa que la ley de la Comunidad Autónoma determine, y será mérito preferente la estancia del candidato en universidades o centros de investigación de reconocido prestigio, españoles o extranjeros, distintos de la universidad que lleve a cabo la contratación.\nb) La finalidad del contrato será la de desarrollar tareas docentes y de investigación.\nc) El contrato será de carácter temporal y con dedicación a tiempo completo.\nd) La duración del contrato no podrá ser inferior a un año ni superior a cinco, pudiendo prorrogarse o renovarse si se hubiera concertado por duración inferior a la máxima, siempre que la duración total no exceda de los indicados cinco años. En cualquier caso, el tiempo total de duración conjunta entre esta figura contractual y la prevista en el artículo anterior, en la misma o distinta universidad, no podrá exceder de ocho años. Las situaciones de incapacidad temporal, maternidad y adopción o acogimiento durante el período de duración del contrato, interrumpirán su cómputo"@es ;
        rdfs:label       "Profesor ayudante doctor"@es , "Profesor Ayudante Doctor"@es , "Assistant Professor Doctor"@en ;
        rdfs:subClassOf  :PDIContratado ;
        roh:country     euCountry:ESP ;
        roh:hasCode     :ES_UNIVERSITY_HR_CODE_ESLPAD ;
        skos:closeMatch  unescothes:C03965 , unescothes:C00015 ;
        skos:inScheme    :ESUniversityHumanResourcesList ;
        skos:notation    "ESLPAD" ;
        skos:prefLabel   "Professor ajudant doctor"@ca , "Profesor ayudante doctor"@ast , "Profesor ayudante doctor"@es , "Profesor axudante doutor"@gl .

:ESUniversityHumanResourcesCodesList
        a               skos:ConceptScheme ;
        rdfs:label      "Códigos dos recursos humanos das universidades de Espanha"@pt , "Códigos dos recursos humanos das universidades de España"@gl , "Códigos de los recursos humanos de les universidaes d'España"@ast , "Codes for the human resources of the universities from Spain"@en , "Codis dels recursos humans de les universitats d'Espanya"@ca , "Códigos de los recursos humanos de las universidades de España"@es , "Codes des resources humains des universités d'Espagne"@fr ;
        skos:prefLabel  "Códigos de los recursos humanos de les universidaes d'España"@ast , "Codis dels recursos humans de les universitats d'Espanya"@ca , "Códigos dos recursos humanos das universidades de Espanha"@pt , "Codes for the human resources of the universities from Spain"@en , "Códigos de los recursos humanos de las universidades de España"@es , "Códigos dos recursos humanos das universidades de España"@gl , "Codes des resources humains des universités d'Espagne"@fr .

:ES_UNIVERSITY_HR_CODE_ESSECGE
        a               skos:Concept ;
        rdfs:label      "ESSECGE" ;
        roh:codeOf     :ES_UNIVERSITY_HR_ESSECGE ;
        skos:inScheme   :ESUniversityHumanResourcesCodesList ;
        skos:prefLabel  "ESSECGE" .

:ProfesorTitularDeUniversidad
        a                owl:Class ;
        rdfs:label       "Profesor titular de universidad"@es , "Profesor Titular de Universidad"@es , "Associate Professor"@en ;
        rdfs:subClassOf  :CuerpoDocente ;
        roh:country     euCountry:ESP ;
        roh:hasCode     :ES_UNIVERSITY_HR_CODE_ESFPTU ;
        skos:closeMatch  unescothes:C00015 , unescothes:C03965 ;
        skos:inScheme    :ESUniversityHumanResourcesList ;
        skos:notation    "ESFPTU" ;
        skos:prefLabel   "Professor titular de universidade"@pt , "Professor titular d'universitat"@ca , "Irakasle titularra"@eu , "Profesor titular d'universidá"@ast , "Professeur titulaire d'université"@fr , "Profesor titular de universidade"@gl , "Profesor titular de universidad"@es .

:ES_UNIVERSITY_HR_ESLPAY
        a                owl:Class ;
        rdfs:label       "Profesor ayudante"@es ;
        rdfs:subClassOf  :PDIContratado ;
        roh:country     euCountry:ESP ;
        roh:hasCode     :ES_UNIVERSITY_HR_CODE_ESLPAY ;
        skos:closeMatch  unescothes:C00015 , unescothes:C03965 ;
        skos:inScheme    :ESUniversityHumanResourcesList ;
        skos:notation    "ESLPAY" ;
        skos:prefLabel   "Profesor axudante"@gl , "Irakasle laguntzailea"@eu , "Profesor ayudante"@ast , "Profesor ayudante"@es , "Professor ajudante"@ca .

:ES_UNIVERSITY_HR_ESRECT
        a                owl:Class ;
        rdfs:label       "Rector"@es ;
        rdfs:subClassOf  vivo:FacultyAdministrativePosition ;
        roh:country     euCountry:ESP ;
        roh:hasCode     :ES_UNIVERSITY_HR_CODE_ESRECT ;
        skos:closeMatch  rohuk:GB_UNIVERSITY_CODE_GBCHAN ;
        skos:inScheme    :ESUniversityHumanResourcesList ;
        skos:notation    "ESRECT" ;
        skos:prefLabel   "Errektorea"@eu , "Rector"@ast , "Rector"@es , "Rector"@gl , "Rector"@ca .

:ES_UNIVERSITY_HR_ESVIREC
        a                owl:Class ;
        rdfs:label       "Vicerrector"@es ;
        rdfs:subClassOf  vivo:FacultyAdministrativePosition ;
        roh:country     euCountry:ESP ;
        roh:hasCode     :ES_UNIVERSITY_HR_CODE_ESVIREC ;
        skos:closeMatch  rohuk:GB_UNIVERSITY_HR_GBCHAN ;
        skos:inScheme    :ESUniversityHumanResourcesList ;
        skos:notation    "ESVIREC" ;
        skos:prefLabel   "Vicerrector"@gl , "Vicerrector"@ast , "Vicerrector"@es , "Errektoreordea"@eu , "Vicerector"@ca .

:ProfesorTitularDeEscuelaUniversitaria
        a                owl:Class ;
        rdfs:label       "Profesor Titular de Escuela Universitaria"@es , "Profesor titular de escuela universitaria"@es , "University School Reader"@en ;
        rdfs:subClassOf  :CuerpoDocente ;
        roh:country     euCountry:ESP ;
        roh:hasCode     :ES_UNIVERSITY_HR_CODE_ESFEU ;
        skos:closeMatch  unescothes:C00015 , unescothes:C03965 ;
        skos:inScheme    :ESUniversityHumanResourcesList ;
        skos:notation    "ESFEU" ;
        skos:prefLabel   "Profesor titular d’escuela universitaria"@ast , "Eskolako irakasle titutarra"@eu , "Profesor titular de escuela universitaria"@es , "Profesor titular de escola universitaria"@gl , "Professor titular d’escola universitària"@ca .

:ES_UNIVERSITY_HR_CODE_ESPASL
        a               skos:Concept ;
        rdfs:label      "ESPASL" ;
        roh:codeOf     :ES_UNIVERSITY_HR_ESPASL ;
        skos:inScheme   :ESUniversityHumanResourcesCodesList ;
        skos:prefLabel  "ESPASL" .

:ES_UNIVERSITY_HR_CODE_ESLPC
        a               skos:Concept ;
        rdfs:label      "ESLPC" ;
        roh:codeOf     :ES_UNIVERSITY_HR_ESLPC ;
        skos:inScheme   :ESUniversityHumanResourcesCodesList ;
        skos:prefLabel  "ESLPC" .

:ES_UNIVERSITY_HR_CODE_ESRECT
        a               skos:Concept ;
        rdfs:label      "ESRECT" ;
        roh:codeOf     :ES_UNIVERSITY_HR_ESRECT ;
        skos:inScheme   :ESUniversityHumanResourcesCodesList ;
        skos:prefLabel  "ESRECT" .

:ES_UNIVERSITY_HR_ESDECA
        a                 owl:Class ;
        rdfs:label        "Decano"@es ;
        rdfs:subClassOf   vivo:FacultyAdministrativePosition ;
        roh:country      euCountry:ESP ;
        roh:hasCode      :ES_UNIVERSITY_HR_CODE_ESDECA ;
        skos:closeMatch  rohuk:GB_UNIVERSITY_HR_GBDEAN ;
        skos:inScheme     :ESUniversityHumanResourcesList ;
        skos:notation     "ESDECA" ;
        skos:prefLabel    "Degà"@ca , "Decano"@gl , "Decano"@es , "Dekanoa"@eu , "Decanu"@ast .

:ES_UNIVERSITY_HR_ESPASF
        a                owl:Class ;
        rdfs:label       "Personal de administración y servicios funcionario"@es ;
        rdfs:subClassOf  vivo:NonAcademicPosition ;
        roh:country     euCountry:ESP ;
        roh:hasCode     :ES_UNIVERSITY_HR_CODE_ESPASF ;
        skos:inScheme    :ESUniversityHumanResourcesList ;
        skos:notation    "ESPASF" ;
        skos:prefLabel   "Personal d'alministración y servicios funcionario"@ast , "Persoal de administración e servizos funcionario"@gl , "Karrerako Funtzionarioak"@eu , "Personal de administración y servicios funcionario"@es , "Personal d’administració i serveis funcionari"@ca .

:ES_UNIVERSITY_HR_CODE_ESLPI
        a               skos:Concept ;
        rdfs:label      "ESLPI" ;
        roh:codeOf     :ES_UNIVERSITY_HR_ESLPI ;
        skos:inScheme   :ESUniversityHumanResourcesCodesList ;
        skos:prefLabel  "ESLPI" .

:ProfesorVisitante  a    owl:Class ;
        rdfs:comment     "La contratación de Profesoras y Profesores Visitantes se ajustará a las siguientes reglas:\na) El contrato se podrá celebrar con profesores o investigadores de reconocido prestigio de otras universidades y centros de investigación, tanto españoles como extranjeros.\nb) La finalidad del contrato será la de desarrollar tareas docentes o investigadoras a través de las que se aporten los conocimientos y la experiencia docente e investigadora de los indicados profesores a la universidad.\nc) El contrato será de carácter temporal con la duración que se acuerde entre las partes y dedicación a tiempo parcial o completo"@es ;
        rdfs:label       "Visiting Professor"@en , "Profesor visitante"@es , "Profesor Visitante"@es ;
        rdfs:subClassOf  :PDIContratado ;
        roh:country     euCountry:ESP ;
        roh:hasCode     :ES_UNIVERSITY_HR_CODE_ESPLV ;
        skos:closeMatch  unescothes:C00015 , unescothes:C03965 ;
        skos:exactMatch  unescothes:C04254 ;
        skos:inScheme    :ESUniversityHumanResourcesList ;
        skos:notation    "ESPLV" ;
        skos:prefLabel   "Irakasle bisitaria"@eu , "Professor visitant"@ca , "Profesor visitante"@ast , "Profesor visitante"@gl , "Profesor visitante"@es .

:ES_UNIVERSITY_HR_CODE_ESPLV
        a               skos:Concept ;
        rdfs:label      "ESPLV" ;
        roh:codeOf     :ProfesorVisitante ;
        skos:inScheme   :ESUniversityHumanResourcesCodesList ;
        skos:prefLabel  "ESPLV" .

:ES_UNIVERSITY_HR_ESPASL
        a                owl:Class ;
        rdfs:label       "Personal de administración y servicios laboral"@es ;
        rdfs:subClassOf  vivo:NonAcademicPosition ;
        roh:country     euCountry:ESP ;
        roh:hasCode     :ES_UNIVERSITY_HR_CODE_ESPASL ;
        skos:inScheme    :ESUniversityHumanResourcesList ;
        skos:notation    "ESPASL" ;
        skos:prefLabel   "Lan kontratudun langile finkoak"@eu , "Persoal de administración e servizos laboral"@gl , "Personal d'alministración y servicios llaboral"@ast , "Personal de administración y servicios laboral"@es , "Personal d’administració i serveis laboral"@ca .

:ES_UNIVERSITY_HR_CODE_ESPLEM
        a               skos:Concept ;
        rdfs:label      "ESPLEM" ;
        roh:codeOf     :ProfesorEmerito ;
        skos:inScheme   :ESUniversityHumanResourcesCodesList ;
        skos:prefLabel  "ESPLEM" .

:ES_UNIVERSITY_HR_CODE_ESFIVEFP
        a               skos:Concept ;
        rdfs:label      "ESFIVEFP" ;
        roh:codeOf     :ES_UNIVERSITY_HR_ESFIVEFP ;
        skos:inScheme   :ESUniversityHumanResourcesCodesList ;
        skos:prefLabel  "ESFIVEFP" .

:ES_UNIVERSITY_HR_CODE_ESLPCD
        a               skos:Concept ;
        rdfs:label      "ESLPCD" ;
        roh:codeOf     :ProfesorContratadoDoctor ;
        skos:inScheme   :ESUniversityHumanResourcesCodesList ;
        skos:prefLabel  "ESLPCD" .

:ES_UNIVERSITY_HR_CODE_ESLPCNP
        a               skos:Concept ;
        rdfs:label      "ESLPCNP" ;
        roh:codeOf     :ES_UNIVERSITY_HR_ESLPCNP ;
        skos:inScheme   :ESUniversityHumanResourcesCodesList ;
        skos:prefLabel  "ESLPCNP" .

:ES_UNIVERSITY_HR_ESLPL
        a                owl:Class ;
        rdfs:label       "Profesor lector"@es ;
        rdfs:subClassOf  :PDIContratado ;
        roh:country     euCountry:ESP ;
        roh:hasCode     :ES_UNIVERSITY_HR_CODE_ESLPL ;
        skos:closeMatch  unescothes:C00015 , unescothes:C03965 ;
        skos:inScheme    :ESUniversityHumanResourcesList ;
        skos:notation    "ESLPL" ;
        skos:prefLabel   "Profesor lector"@gl , "Profesor lector"@ast , "Profesor lector"@es , "Professor lector"@ca , "Irakurlea"@eu .

:ES_UNIVERSITY_HR_CODE_ESVIDEC
        a               skos:Concept ;
        rdfs:label      "ESVIDEC" ;
        roh:codeOf     :ES_UNIVERSITY_HR_ESVIDEC ;
        skos:inScheme   :ESUniversityHumanResourcesCodesList ;
        skos:prefLabel  "ESVIDEC" .

:CuerpoDocente  a         owl:Class ;
        rdfs:comment      "Personal funcionario o permanente de una universidad."@es ;
        rdfs:label        "Cuerpo Docente"@es , "Faculty"@en ;
        rdfs:subClassOf   vivo:FacultyPosition ;
        owl:disjointWith  :PDIContratado .

:ES_UNIVERSITY_HR_CODE_ESLPCP
        a               skos:Concept ;
        rdfs:label      "ESLPCP" ;
        roh:codeOf     :ES_UNIVERSITY_HR_ESLPCP ;
        skos:inScheme   :ESUniversityHumanResourcesCodesList ;
        skos:prefLabel  "ESLPCP" .

:ES_UNIVERSITY_HR_CODE_ESFPCU
        a               skos:Concept ;
        rdfs:label      "ESFPCU" ;
        roh:codeOf     :CatedraticoDeUniversidad ;
        skos:inScheme   :ESUniversityHumanResourcesCodesList ;
        skos:prefLabel  "ESFPCU" .

:ES_UNIVERSITY_HR_ESSECGE
        a                owl:Class ;
        rdfs:label       "Secretario general"@es ;
        rdfs:subClassOf  vivo:FacultyAdministrativePosition ;
        roh:country     euCountry:ESP ;
        roh:hasCode     :ES_UNIVERSITY_HR_CODE_ESSECGE ;
        skos:inScheme    :ESUniversityHumanResourcesList ;
        skos:notation    "ESSECGE" ;
        skos:prefLabel   "Secretario general"@es , "Secretariu xeneral"@ast , "Idazkari Nagusia"@eu , "Secretari general"@ca , "Secretario xeral"@gl .

:ES_UNIVERSITY_HR_CODE_ESFPTN
        a               skos:Concept ;
        rdfs:label      "ESFPTN" ;
        roh:codeOf     :ES_UNIVERSITY_HR_ESFPTN ;
        skos:inScheme   :ESUniversityHumanResourcesCodesList ;
        skos:prefLabel  "ESFPTN" .

:ES_UNIVERSITY_HR_CODE_ESLPADJ
        a               skos:Concept ;
        rdfs:label      "ESLPADJ" ;
        roh:codeOf     :ES_UNIVERSITY_HR_ESLPADJ ;
        skos:inScheme   :ESUniversityHumanResourcesCodesList ;
        skos:prefLabel  "ESLPADJ" .

:ES_UNIVERSITY_HR_CODE_ESVIREC
        a               skos:Concept ;
        rdfs:label      "ESVIREC" ;
        roh:codeOf     :ES_UNIVERSITY_HR_ESVIREC ;
        skos:inScheme   :ESUniversityHumanResourcesCodesList ;
        skos:prefLabel  "ESVIREC" .

:ES_UNIVERSITY_HR_CODE_ESJEFDEP
        a               skos:Concept ;
        rdfs:label      "ESJEFDEP" ;
        roh:codeOf     :ES_UNIVERSITY_HR_ESJEFDEP ;
        skos:inScheme   :ESUniversityHumanResourcesCodesList ;
        skos:prefLabel  "ESJEFDEP" .

:ES_UNIVERSITY_HR_CODE_ESLPAG
        a               skos:Concept ;
        rdfs:label      "ESLPAG" ;
        roh:codeOf     :ES_UNIVERSITY_HR_ESLPAG ;
        skos:inScheme   :ESUniversityHumanResourcesCodesList ;
        skos:prefLabel  "ESLPAG" .

:ES_UNIVERSITY_HR_ESLI
        a                owl:Class ;
        rdfs:label       "Investigador"@es ;
        rdfs:subClassOf  vivo:NonFacultyAcademicPosition ;
        roh:country     euCountry:ESP ;
        roh:hasCode     :ES_UNIVERSITY_HR_CODE_ESLI ;
        skos:closeMatch  unescothes:C03376 ;
        skos:inScheme    :ESUniversityHumanResourcesList ;
        skos:notation    "ESLI" ;
        skos:prefLabel   "Investigador"@ast , "Investigador"@es , "Investigador"@gl , "Investigador"@ca , "Ikertzaileak"@eu .

:CatedraticoDeUniversidad
        a                owl:Class ;
        rdfs:label       "University Professor"@en , "Profesor catedrático de universidad"@es , "Catedrático de Universidad"@es ;
        rdfs:subClassOf  :CuerpoDocente ;
        roh:country     euCountry:ESP ;
        roh:hasCode     :ES_UNIVERSITY_HR_CODE_ESFPCU ;
        skos:closeMatch  unescothes:C00015 , unescothes:C03965 ;
        skos:inScheme    :ESUniversityHumanResourcesList ;
        skos:notation    "ESFPCU" ;
        skos:prefLabel   "Professeur d'université"@fr , "Professor catedrático de universidade"@pt , "Profesor catedrático de universidad"@es , "Profesor catedrático de universidade"@gl , "Professor catedràtic d'universitat"@ca , "Profesor catedráticu d'universidá"@ast , "Unibertsitateko katedraduna"@eu .

:ES_UNIVERSITY_HR_CODE_ESFEU
        a               skos:Concept ;
        rdfs:label      "ESFEU" ;
        roh:codeOf     :ProfesorTitularDeEscuelaUniversitaria ;
        skos:inScheme   :ESUniversityHumanResourcesCodesList ;
        skos:prefLabel  "ESFEU" .

:ESUniversityHumanResourcesList
        a               skos:ConceptScheme ;
        rdfs:label      "Recursos humanos de les universidaes d'España"@ast , "Resources humains des universités d'Espagne"@fr , "Human resources of the universities from Spain"@en , "Recursos humans de les universitats d'Espanya"@ca , "Recursos humanos de las universidades de España"@es , "Recursos humanos das universidades de Espanha"@pt , "Recursos humanos das universidades de España"@gl ;
        skos:prefLabel  "Human resources of the universities from Spain"@en , "Recursos humanos das universidades de Espanha"@pt , "Recursos humanos de les universidaes d'España"@ast , "Recursos humanos das universidades de España"@gl , "Resources humains des universités d'Espagne"@fr , "Recursos humanos de las universidades de España"@es , "Recursos humans de les universitats d'Espanya"@ca .

:ES_UNIVERSITY_HR_CODE_ESLPAM
        a               skos:Concept ;
        rdfs:label      "ESLPAM" ;
        roh:codeOf     :ES_UNIVERSITY_HR_ESLPAM ;
        skos:inScheme   :ESUniversityHumanResourcesCodesList ;
        skos:prefLabel  "ESLPAM" .

:ProfesorAsociado  a     owl:Class ;
        rdfs:comment     "La contratación de Profesoras y Profesores Asociados se ajustará a las siguientes reglas:\na) El contrato se podrá celebrar con especialistas de reconocida competencia que acrediten ejercer su actividad profesional fuera del ámbito académico universitario.\nb) La finalidad del contrato será la de desarrollar tareas docentes a través de las que se aporten sus conocimientos y experiencia profesionales a la universidad.\nc) El contrato será de carácter temporal y con dedicación a tiempo parcial.\nd) La duración del contrato será trimestral, semestral o anual, y se podrá renovar por períodos de igual duración, siempre que se siga acreditando el ejercicio de la actividad profesional fuera del ámbito académico universitario."@es ;
        rdfs:label       "Profesor asociado"@es , "Associate Professor"@en , "Profesor Asociado"@es ;
        rdfs:subClassOf  :PDIContratado ;
        roh:country     euCountry:ESP ;
        roh:hasCode     :ES_UNIVERSITY_HR_CODE_ESLPAS ;
        skos:closeMatch  "C03965" ;
        skos:closeMatch  unescothes:C00015 ;
        skos:inScheme    :ESUniversityHumanResourcesList ;
        skos:notation    "ESLPAS" ;
        skos:prefLabel   "Profesor asociado"@gl , "Irakasle elkartua"@eu , "Profesor asociáu"@ast , "Professor associat"@ca , "Profesor asociado"@es .

:ES_UNIVERSITY_HR_ESLPCNP
        a                owl:Class ;
        rdfs:label       "Profesor colaborador no permanente"@es ;
        rdfs:subClassOf  :PDIContratado ;
        roh:country     euCountry:ESP ;
        roh:hasCode     :ES_UNIVERSITY_HR_CODE_ESLPCNP ;
        skos:closeMatch  unescothes:C03965 , unescothes:C00015 ;
        skos:inScheme    :ESUniversityHumanResourcesList ;
        skos:notation    "ESLPCNP" ;
        skos:prefLabel   "Unibertsitateko kolaboratzailea (Ez--iraunkorra)"@eu , "Profesor colaborador no permanente"@es , "Profesor colaborador non permanente"@gl , "Professor col·laborador no permanent"@ca , "Profesor collaborador non permanente"@ast .

:ES_UNIVERSITY_HR_CODE_ESFPCEU
        a               skos:Concept ;
        rdfs:label      "ESFPCEU" ;
        roh:codeOf     :CatedraticoDeEscuelaUniversitaria ;
        skos:inScheme   :ESUniversityHumanResourcesCodesList ;
        skos:prefLabel  "ESFPCEU" .

:ES_UNIVERSITY_HR_CODE_ESLPL
        a               skos:Concept ;
        rdfs:label      "ESLPL" ;
        roh:codeOf     :ES_UNIVERSITY_HR_ESLPL ;
        skos:inScheme   :ESUniversityHumanResourcesCodesList ;
        skos:prefLabel  "ESLPL" .

:ES_UNIVERSITY_HR_ESLPCP
        a                owl:Class ;
        rdfs:label       "Profesor colaborador permanente"@es ;
        rdfs:subClassOf  :CuerpoDocente ;
        roh:country     euCountry:ESP ;
        roh:hasCode     :ES_UNIVERSITY_HR_CODE_ESLPCP ;
        skos:closeMatch  unescothes:C00015 , unescothes:C03965 ;
        skos:inScheme    :ESUniversityHumanResourcesList ;
        skos:notation    "ESLPCP" ;
        skos:prefLabel   "Unibertsitateko kolaboratzailea (Iraunkorra)"@eu , "Profesor collaborador permanente"@ast , "Profesor colaborador permanente"@es , "Profesor colaborador permanente"@gl , "Professor col·laborador permanent"@ca .

:CatedraticoDeEscuelaUniversitaria
        a                owl:Class ;
        rdfs:label       "Catedrático de Escuela Universitaria"@es , "University School Professor"@en , "Profesor catedrático de escuela universitaria"@es ;
        rdfs:subClassOf  :CuerpoDocente ;
        roh:country     euCountry:ESP ;
        roh:hasCode     :ES_UNIVERSITY_HR_CODE_ESFPCEU ;
        skos:closeMatch  unescothes:C00015 , unescothes:C03965 ;
        skos:inScheme    :ESUniversityHumanResourcesList ;
        skos:notation    "ESFPCEU" ;
        skos:prefLabel   "Profesor catedrático de escuela universitaria"@es , "Unibertsitateko Eskolako Katedraduna"@eu , "Profesor catedrático de escola universitaria"@gl , "Profesor catedráticu d'escuela universitaria"@ast , "Professor catedràtic d’escola universitària"@ca .

:ES_UNIVERSITY_HR_ESFPTN
        a                 owl:Class ;
        rdfs:label        "Profesor titular de escuela de náutica"@es ;
        rdfs:subClassOf   :CuerpoDocente ;
        roh:country      euCountry:ESP ;
        roh:geoDivision  geo:ES_DIVISION_LEVEL_1_ES_PV ;
        roh:hasCode      :ES_UNIVERSITY_HR_CODE_ESFPTN ;
        skos:closeMatch   unescothes:C03965 , unescothes:C00015 ;
        skos:inScheme     :ESUniversityHumanResourcesList ;
        skos:notation     "ESFPTN" ;
        skos:prefLabel    "Professor titular d'escola de nàutica"@ca , "Nautika Eskola Ofizialeko Irakasle numerarioa"@eu , "Profesor oficial d'escuela de náutica"@ast , "Profesor titular de escuela de náutica"@es , "Profesor titular de escola de náutica"@gl .

:ES_UNIVERSITY_HR_CODE_ESLPAS
        a               skos:Concept ;
        rdfs:label      "ESLPAS" ;
        roh:codeOf     :ProfesorAsociado ;
        skos:inScheme   :ESUniversityHumanResourcesCodesList ;
        skos:prefLabel  "ESLPAS" .

:ES_UNIVERSITY_HR_ESFIVEFNP
        a                 owl:Class ;
        rdfs:label        "Profesor Ivef no permanente"@es ;
        rdfs:subClassOf   :PDIContratado ;
        roh:country      euCountry:ESP ;
        roh:geoDivision  geo:ES_DIVISION_LEVEL_1_ES_PV ;
        roh:hasCode      :ES_UNIVERSITY_HR_CODE_ESFIVEFNP ;
        skos:closeMatch   unescothes:C00015 ;
        skos:inScheme     :ESUniversityHumanResourcesList ;
        skos:notation     "ESFIVEFNP" ;
        skos:prefLabel    "SHEE Iraskaslea (Ez--Iraunkorra)"@eu , "Professor Ivef no permanent"@ca , "Profesor Ivef no permanente"@gl , "Profesor Ivef no permanente"@ast , "Profesor Ivef no permanente"@es .

:ES_UNIVERSITY_HR_ESLPAG
        a                owl:Class ;
        rdfs:label       "Profesor agregado"@es ;
        rdfs:subClassOf  :CuerpoDocente ;
        roh:country     euCountry:ESP ;
        roh:hasCode     :ES_UNIVERSITY_HR_CODE_ESLPAG ;
        skos:closeMatch  unescothes:C00015 , unescothes:C03965 ;
        skos:inScheme    :ESUniversityHumanResourcesList ;
        skos:notation    "ESLPAG" ;
        skos:prefLabel   "Profesor agregado"@gl , "Profesor agregado"@es , "Profesor agregáu"@ast , "Irakasle agregatua"@eu , "Professor agregat"@ca .

:ProfesorEmerito  a      owl:Class ;
        rdfs:comment     "Las universidades, de acuerdo con sus estatutos, podrán nombrar a Profesores Eméritos entre profesoras y profesores jubilados que hayan prestado servicios destacados a la universidad"@es ;
        rdfs:label       "Professor Emeritus"@en , "Profesor Emérito"@es , "Profesor emérito"@es ;
        rdfs:subClassOf  :PDIContratado ;
        roh:country     euCountry:ESP ;
        roh:hasCode     :ES_UNIVERSITY_HR_CODE_ESPLEM ;
        skos:closeMatch  unescothes:C00015 , unescothes:C03965 , rohpt:PT_UNIVERSITY_HR_PTPEM ;
        skos:inScheme    :ESUniversityHumanResourcesList ;
        skos:notation    "ESPLEM" ;
        skos:prefLabel   "Profesor emérito"@es , "Profesor emérito"@gl , "Profesor eméritu"@ast , "Irakasle emeritua"@eu , "Professor emèrit"@ca .

:ProfesorContratadoDoctor
        a                owl:Class ;
        rdfs:comment     "La contratación de Profesoras y Profesores Contratados Doctores se ajustará a las siguientes reglas:\na) El contrato se celebrará con doctores que reciban la evaluación positiva por parte de la Agencia Nacional de Evaluación de la Calidad y Acreditación o del órgano de evaluación externo que la ley de la Comunidad Autónoma determine.\nb) La finalidad del contrato será la de desarrollar, con plena capacidad docente e investigadora, tareas de docencia y de investigación, o prioritariamente de investigación.\nc) El contrato será de carácter indefinido y con dedicación a tiempo completo."@es ;
        rdfs:label       "Hired Professor Doctorr"@en , "Profesor contratado doctor"@es , "Profesor Contratado Doctor"@es ;
        rdfs:subClassOf  :PDIContratado ;
        roh:country     euCountry:ESP ;
        roh:hasCode     :ES_UNIVERSITY_HR_CODE_ESLPCD ;
        skos:closeMatch  unescothes:C03965 , unescothes:C00015 ;
        skos:inScheme    :ESUniversityHumanResourcesList ;
        skos:notation    "ESLPCD" ;
        skos:prefLabel   "Profesor contratado doctor"@es , "Profesor contratado doutor"@gl , "Professor contractat doctor"@ca , "Profesor contratáu doctor"@ast .

:PDIContratado  a        owl:Class ;
        rdfs:comment     "Personal temporal de una universidad."@es ;
        rdfs:label       "Hired PDI"@en , "PDI Contratado"@es ;
        rdfs:subClassOf  vivo:FacultyPosition .

:ES_UNIVERSITY_HR_ESLPADJ
        a                owl:Class ;
        rdfs:label       "Profesor adjunto"@es ;
        rdfs:subClassOf  :PDIContratado ;
        roh:country     euCountry:ESP ;
        roh:hasCode     :ES_UNIVERSITY_HR_CODE_ESLPADJ ;
        skos:closeMatch  unescothes:C00015 , unescothes:C03965 ;
        skos:inScheme    :ESUniversityHumanResourcesList ;
        skos:notation    "ESLPADJ" ;
        skos:prefLabel   "Professor adjunt"@ca , "Profesor adxuntu"@ast , "Profesor adxunto"@gl , "Irakasle atxikia"@eu , "Profesor adjunto"@es .

:ES_UNIVERSITY_HR_CODE_ESFPTU
        a               skos:Concept ;
        rdfs:label      "ESFPTU" ;
        roh:codeOf     :ProfesorTitularDeUniversidad ;
        skos:inScheme   :ESUniversityHumanResourcesCodesList ;
        skos:prefLabel  "ESFPTU" .

:Ayudante  a             owl:Class ;
        rdfs:comment     "Los ayudantes serán contratados entre quienes hayan superado todas las materias de estudio que se determinen en los criterios a que hace referencia el artículo 38 y con la finalidad principal de completar su formación investigadora. La contratación será con dedicación a tiempo completo, por una duración no superior a cuatro años improrrogables. Los ayudantes también podrán colaborar en tareas docentes en los términos que establezcan los Estatutos."@es ;
        rdfs:label       "Assistant"@en , "Ayudante"@es ;
        rdfs:subClassOf  :PDIContratado .

:ES_UNIVERSITY_HR_ESLPC
        a                 owl:Class ;
        rdfs:label        "Profesor catedrático laboral"@es ;
        rdfs:subClassOf   :CuerpoDocente ;
        roh:country      euCountry:ESP ;
        roh:geoDivision  geo:ES_DIVISION_LEVEL_1_ES_CT ;
        roh:hasCode      :ES_UNIVERSITY_HR_CODE_ESLPC ;
        skos:closeMatch   unescothes:C03965 , unescothes:C00015 ;
        skos:inScheme     :ESUniversityHumanResourcesList ;
        skos:notation     "ESLPC" ;
        skos:prefLabel    "Profesor catedrático laboral"@gl , "Profesor catedrático laboral"@es , "Professor catedràtic laboral"@ca , "Profesor catedráticu llaboral"@ast .

:ES_UNIVERSITY_HR_CODE_ESLPAY
        a               skos:Concept ;
        rdfs:label      "ESLPAY" ;
        roh:codeOf     :ES_UNIVERSITY_HR_ESLPAY ;
        skos:inScheme   :ESUniversityHumanResourcesCodesList ;
        skos:prefLabel  "ESLPAY" .

:ES_UNIVERSITY_HR_ESLPAM
        a                owl:Class ;
        rdfs:label       "Profesor asociado médico"@es ;
        rdfs:subClassOf  :PDIContratado ;
        roh:country     euCountry:ESP ;
        roh:hasCode     :ES_UNIVERSITY_HR_CODE_ESLPAM ;
        skos:closeMatch  unescothes:C00015 , unescothes:C03965 ;
        skos:inScheme    :ESUniversityHumanResourcesList ;
        skos:notation    "ESLPAM" ;
        skos:prefLabel   "Professor associat mèdic"@ca , "Profesor asociado médico"@gl , "Profesor asociado médico"@es , "Profesor asociáu mélicu"@ast .


:ES_UNIVERSITY_HR_CODE_ESFIVEFNP
        a               skos:Concept ;
        rdfs:label      "ESFIVEFNP" ;
        roh:codeOf     :ES_UNIVERSITY_HR_ESFIVEFNP ;
        skos:inScheme   :ESUniversityHumanResourcesCodesList ;
        skos:prefLabel  "ESFIVEFNP" .

:ES_UNIVERSITY_HR_CODE_ESLI
        a               skos:Concept ;
        rdfs:label      "ESLI" ;
        roh:codeOf     :ES_UNIVERSITY_HR_ESLI ;
        skos:inScheme   :ESUniversityHumanResourcesCodesList ;
        skos:prefLabel  "ESLI" .

:ES_UNIVERSITY_HR_CODE_ESDECA
        a               skos:Concept ;
        rdfs:label      "ESDECA" ;
        roh:codeOf     :ES_UNIVERSITY_HR_ESDECA ;
        skos:inScheme   :ESUniversityHumanResourcesCodesList ;
        skos:prefLabel  "ESDECA" .

